General Relativity 05

> Reference: [UCI OpenCourseWare - GR 06](https://www.youtube.com/watch?v=90KT6nW-cIc&list=PLqOZ6FD_RQ7ln1ZQPEU9aZQsEj0eyGlT6&indx=7) ([Playlist](https://www.youtube.com/playlist?list=PLqOZ6FD_RQ7ln1ZQPEU9aZQsEj0eyGlT6))

### Equation of free fall from Lagrangian

Last time we wrote down the equation of free fall:
$$
\frac{d^2x^\lambda}{d\tau^2} + \Gamma^\lambda{}_{\mu\nu}\frac{dx^\mu}{d\tau}\frac{dx^\nu}{d\tau}=0\\
\\
\text{or}\\
\\
g_{\lambda\sigma}\frac{d^2x^\sigma}{d\tau^2} + \Gamma_{\lambda\mu\nu}\frac{dx^\mu}{d\tau}\frac{dx^\nu}{d\tau}=0
$$
where $\Gamma$ is the Christoffel symbol of the first kind, which can be written as a function of metric tensor:
$$
\Gamma_{\lambda\mu\nu} = \frac 12 \left(
  \frac{\partial g_{\nu\lambda}}{\partial x^\mu} +
  \frac{\partial g_{\mu\lambda}}{\partial x^\nu} -
  \frac{\partial g_{\mu\nu}}{\partial x^\lambda}
\right)
$$

Today we are going to derive the equation of free fall from the variational principal.

Action:
$$
A = \int_A^Bd\tau\\
$$
the principal is that the equation of motion can be derived from:
$$
\delta A = 0
$$
By this, it means a particle goes from $A$ to $B$ from a trajectory $x^\mu(p)$ where $p \in [0, 1]$ is an parameter. If we perturb the trajectory with an arbitrary finite variation $x^\mu(p)$ multiply by an infinitesimal factor of $\Delta$, then the action remains the same. We can write it down:
$$\begin{align*}
\delta \int_A^Bd\tau &= \delta \int_A^Bdp \frac{d\tau}{dp}\\
\\
d\tau^2&=-g_{\mu\nu}dx^\mu dx^\nu \\
\delta d\tau&=\delta\sqrt{-g_{\mu\nu}dx^\mu dx^\nu} \\
&=\frac{1}{2d\tau}\delta(-g_{\mu\nu}dx^\mu dx^\nu) \\
&=\frac{1}{2d\tau}(
  -\delta g_{\mu\nu}dx^\mu dx^\nu
  -g_{\mu\nu}\left(
    d\delta x^\mu dx^\nu +
    dx^\mu d\delta x^\nu
  \right)
) \\
&=\frac{1}{2d\tau}(
  -\frac{\partial g_{\mu\nu}}{\partial x^\lambda}\delta x^\lambda dx^\mu dx^\nu
  -g_{\mu\nu}d\delta x^\mu dx^\nu
  -g_{\mu\nu}dx^\mu d\delta x^\nu
) \\
\end{align*}$$

The boundary term is $0$ and integrate by partial:

$$\begin{align*}

-g_{\mu\nu}d\delta x^\mu dx^\nu
&\to
d(g_{\mu\nu}dx^\nu) \delta x^\mu
\\
&=
(dg_{\mu\nu}dx^\nu + g_{\mu\nu}d^2x^\nu) \delta x^\mu
\\
&=
(dg_{\lambda\nu}dx^\nu + g_{\lambda\nu}d^2x^\nu) \delta x^\lambda
\\
&=
\left(
  \frac{\partial g_{\lambda\nu}}{\partial x^\mu}dx^\mu dx^\nu + g_{\lambda\sigma}d^2x^\sigma
\right) \delta x^\lambda
\\
\\
-g_{\mu\nu}dx^\mu d\delta x^\nu
&=
\left(
  \frac{\partial g_{\lambda\mu}}{\partial x^\nu}dx^\mu dx^\nu + g_{\lambda\sigma}d^2x^\sigma
\right) \delta x^\lambda
\\

\end{align*}$$

Plug it in,

$$\begin{align*}
\delta d\tau
&\to
\frac{1}{2d\tau}\left(
  -\frac{\partial g_{\mu\nu}}{\partial x^\lambda}dx^\mu dx^\nu
  +
  \frac{\partial g_{\lambda\nu}}{\partial x^\mu}dx^\mu dx^\nu
  +
  \frac{\partial g_{\lambda\mu}}{\partial x^\nu}dx^\mu dx^\nu +
  2g_{\lambda\sigma}d^2x^\sigma
\right)\delta x^\lambda \\

&=
\frac{1}{d\tau}\left(
  \Gamma_{\lambda\mu\nu}dx^\mu dx^\nu +
  g_{\lambda\sigma}d^2x^\sigma
\right)\delta x^\lambda \\
&=
\left(
  \Gamma_{\lambda\mu\nu} \frac{dx^\mu}{d\tau} \frac{dx^\nu}{d\tau} +
  g_{\lambda\sigma}\frac{d^2x^\sigma}{d\tau^2}
\right)\delta x^\lambda \\

\end{align*}$$

<hr/>

$$\begin{align*}
0 = \delta \int_A^Bd\tau
&= \int_A^Bd\tau \left(
  \Gamma_{\lambda\mu\nu} \frac{dx^\mu}{d\tau} \frac{dx^\nu}{d\tau} +
  g_{\lambda\sigma}\frac{d^2x^\sigma}{d\tau^2}
\right)\delta x^\lambda\\
\end{align*}$$

Since $\delta x^\lambda$ is arbitrary, we get again the equation of free fall:
$$
\Gamma_{\lambda\mu\nu} \frac{dx^\mu}{d\tau} \frac{dx^\nu}{d\tau} +
  g_{\lambda\sigma}\frac{d^2x^\sigma}{d\tau^2} = 0
$$

By definition, this is trajectory of the stationary path (in terms of proper time) in 4 dimentional spacetime. This is the **Geodesics**. Therefore we replaced gravitational force with the geometry of spacetime.

There has a clear consequence with QM because of path integral:
$$
Amp(A\to B)\propto \int d \exp\left({\frac{i}{\hbar} \int d\tau mc^2A}\right)
$$

---

### Newtonian approximation

For slow moving particles:
$$\begin{align*}
\frac{d^2x^\lambda}{d\tau^2} + \Gamma^\lambda{}_{\mu\nu}\frac{dx^\mu}{d\tau}\frac{dx^\nu}{d\tau}&\approx
\frac{d^2x^\lambda}{dt^2}\left(\frac{dt}{d\tau}\right)^2 + \Gamma^\lambda{}_{00}\left(\frac{dt}{d\tau}\right)^2\\
\frac{d^2x^\lambda}{dt^2} + \Gamma^\lambda{}_{00} &\approx 0
\end{align*}$$

For weak, stationary fields:
$$\begin{align*}
g_{\alpha\beta} &=\eta_{\alpha\beta}+h_{\alpha\beta},\quad\quad|h_{\alpha\beta}| \ll 1\,,\dot h = 0\\
g^{\alpha\gamma} &=\eta^{\alpha\gamma}+h'^{\alpha\gamma} \\
g^{\alpha\gamma}g_{\alpha\beta}&=
\delta^\gamma{}_\beta+\eta^{\alpha\gamma}h_{\alpha\beta}+\eta_{\alpha\beta}h'^{\alpha\gamma}+o(h^2)\\
0 &= \eta^{\alpha\gamma}h_{\alpha\beta}+\eta_{\alpha\beta}h'^{\alpha\gamma}\\
&=h^\gamma{}_{\beta}+h'^\gamma{}_{\beta}\\
g^{\alpha\gamma} &= \eta^{\alpha\beta}-h^{\alpha\beta}\\
\\
\Gamma^{\lambda}{}_{00}&\approx\frac{1}{2}\eta^{\sigma\lambda}(
  \partial_0 g_{\sigma 0} + \partial_0 g_{\sigma 0} - \partial_\sigma g_{0 0}
)\\
&=\frac{1}{2}\eta^{\sigma\lambda}(
  \partial_0 h_{\sigma 0} + \partial_0 h_{\sigma 0} - \partial_\sigma h_{0 0}
)\\
&=-\frac{1}{2}\eta^{\sigma\lambda}\partial_\sigma h_{0 0}\\
&=-\frac{1}{2}(0, \vec\nabla h_{0 0})^\lambda\\
\end{align*}$$

<hr/>

If both conditions are met:

$$
\vec{a}= \frac{1}{2}\vec\nabla h_{0 0}
$$

This looks a lot like the the Newtonian gravitation:
$$
\vec{a} = -\vec\nabla \phi
$$
where $\phi$ is the gravitational potential (which is always negative),
$$
h_{00} = -2\phi + const
$$
At the boundary, the gravitation field is $0$, the $h_{00}$ should also be $0$, therefore the constant should be $0$ as well.
$$
h_{00} = -2\phi
$$
$$\begin{align*}
\phi &= -\frac{mG}{|r|}\\
g_{00} &= -1-2\phi\\
&= \frac{2mG}{|r|}-1
\end{align*}$$

Remark: 1. $g_{00}$ goes to $0$ at the event horizon. 2. The boundary gravitational field may not be $0$.

---

In the case of stronger gravitational field $\phi$ (which is dimensionless):

1. $10^{-4}$ at the surface of a white dwarf;
2. $10^{-6}$ at the surface of the sun;
2. $10^{-9}$ at the surface of the earth;
2. $10^{-39}$ at the surface of an proton;

--

### Time Dilation

$$
d\tau = \sqrt{-\eta_{\alpha\beta} d\xi^\alpha d\xi^\beta}
= \sqrt{-g_{\alpha\beta} dx^\alpha dx^\beta}
$$
We can caluculate $dt/d\tau$ which is the factor of time dilation:
$$\begin{align*}
\frac{dt}{d\tau}&=\left(-g_{\alpha\beta} \frac{dx^\alpha}{dt} \frac{dx^\beta}{dt}\right)^{-\frac 12}\\
\frac{dx^\mu}{dt} &= (1, \vec v)\\
\end{align*}$$

If the $\vec v=0$:
$$
\frac{dt}{d\tau} = \frac{1}{\sqrt{-g_{00}}}
$$

comparing two clocks:
$$
\frac{dt_1}{dt_2} = \frac{\sqrt{-g_{00}(x_2)}}{\sqrt{-g_{00}(x_1)}}
$$
The frequency of the two stationary clock:
$$
\frac{dv_2}{dv_1} = \frac{\sqrt{-g_{00}(x_2)}}{\sqrt{-g_{00}(x_1)}}
$$

In the previous conditions:

$$\begin{align*}
\frac{dv_2}{dv_1} &\approx 1 + \phi(x_2) - \phi(x_1) \\
&= 1 + MG \frac{|r_1| - |r_2|}{|r_2r_1|} \\
\end{align*}$$
